theories/Subst.v
@@ -5,90 +5,181 @@ From Lang Require Import
   FreeVariables
   Invert
   Partition
-  SplitRemove
   StructuralFreeVariables
   StructuralHole
   StructuralSubst
   Terms.
+
+Fixpoint checked_sub this_much from :=
+  match this_much with
+  | O => Some from
+  | S n =>
+      match from with
+      | O => None
+      | S m => checked_sub n m
+      end
+  end.
+
+Example checked_sub_3_5 : checked_sub 3 5 = Some 2. Proof. reflexivity. Qed.
+Example checked_sub_5_3 : checked_sub 5 3 = None. Proof. reflexivity. Qed.
 
 Fixpoint subst_hole_acc acc x t :=
   match t with
   | TmVoid
   | TmStar _
   | TmAtom _ =>
-      (SHoleTerm t, acc)
+      (SHoleTerm t, match acc with None => None | Some _ => Some O end)
   | TmVarS z =>
       if eqb z x then
         match acc with
         (* no shadowing *)
         | Some O => (SHoleHere, None)
         (* shadowed *)
-        | Some (S n) => (SHoleTerm t, Some n)
+        | Some (S n) => (SHoleTerm t, Some 1)
         (* already used *)
         | None => (SHoleTerm t, None)
         end
       else
-        (SHoleTerm t, acc)
+        (SHoleTerm t, match acc with None => None | Some _ => Some O end)
   | TmPack id arg ty curry =>
-      let (scurry, ac1) := subst_hole_acc (if eq_opt arg (Some x) then option_map S acc else acc) x curry in
-      (SHolePack id arg (structural_subst_hole x ty) scurry, ac1)
+      let shadow := if eq_opt arg (Some x) then option_map S acc else acc in
+      let (scurry, ac1) := subst_hole_acc shadow x curry in
+      (SHolePack id arg (match acc with Some O => structural_subst_hole x ty | _ => SHoleTerm ty end) scurry, ac1)
   | TmForA arg ty body =>
-      let (sbody, ac1) := subst_hole_acc (if eq_opt arg (Some x) then option_map S acc else acc) x body in
-      (SHoleForA arg (structural_subst_hole x ty) sbody, ac1)
+      let shadow := if eq_opt arg (Some x) then option_map S acc else acc in
+      let (sbody, ac1) := subst_hole_acc shadow x body in
+      (SHoleForA arg (match acc with Some O => structural_subst_hole x ty | _ => SHoleTerm ty end) sbody, ac1)
   | TmAppl f z =>
-      let (sf, ac1) := subst_hole_acc acc x f in
-      let (sz, ac2) := subst_hole_acc ac1 x z in
-      (SHoleAppl sf sz, ac2)
+      let (sf, tmp) := subst_hole_acc acc x f in
+      (* `tmp` represents the number of shadowed instances that `f` consumed *)
+      let acc' := match tmp with None => None | Some n => match acc with None => None | Some m => checked_sub n m end end in
+      let (sz, out) := subst_hole_acc acc' x z in
+      (SHoleAppl sf sz, out)
   end.
 Definition subst_hole := subst_hole_acc (Some O).
 Arguments subst_hole/ x t.
 Definition subst x y t := sfill (fst (subst_hole x t)) y.
 Arguments subst/ x y t.
 
-Example subst_simple_f : forall f x, (* note that we don't require `f <> x` *)
-  subst f TmVoid (TmAppl (TmVarS f) (TmVarS x)) = TmAppl TmVoid (TmVarS x).
+Example subst_simple_f : forall f x y, (* note that we don't require `f <> x` *)
+  (* subst f y (f x) = y x *)
+  subst f y (TmAppl (TmVarS f) (TmVarS x)) = TmAppl y (TmVarS x).
 Proof. intros. simpl. rewrite eqb_refl. destruct (eqb x f); reflexivity. Qed.
 
-Example subst_simple_x : forall f x, f <> x ->
-  subst x TmVoid (TmAppl (TmVarS f) (TmVarS x)) = TmAppl (TmVarS f) TmVoid.
-Proof. intros. simpl. apply eqb_neq in H. rewrite H. rewrite eqb_refl. reflexivity. Qed.
+Example subst_simple_x : forall f x y, f <> x ->
+  (* subst x y (f x) = f y *)
+  subst x y (TmAppl (TmVarS f) (TmVarS x)) = TmAppl (TmVarS f) y.
+Proof. intros. simpl. apply eqb_neq in H. rewrite H. rewrite eqb_refl. simpl. reflexivity. Qed.
 
-Example subst_lambda_t : forall t x, x <> t ->
-  subst t TmVoid (TmForA (Some x) (TmVarS t) (TmAppl (TmVarS x) (TmVarS x))) =
-  TmForA (Some x) TmVoid (TmAppl (TmVarS x) (TmVarS x)).
-Proof. intros. simpl. apply eqb_neq in H. rewrite H. simpl. rewrite eqb_refl. reflexivity. Qed.
+Example subst_lambda_t : forall t x y, x <> t ->
+  (* subst t y (\x:t. x x) = \x:y. x x *)
+  subst t y (TmForA (Some x) (TmVarS t) (TmAppl (TmVarS x) (TmVarS x))) =
+  TmForA (Some x) y (TmAppl (TmVarS x) (TmVarS x)).
+Proof. intros. simpl. apply eqb_neq in H. rewrite H. simpl. rewrite eqb_refl. simpl. reflexivity. Qed.
 
-Example subst_lambda_x : forall t x, t <> x ->
-  subst x TmVoid (TmForA (Some x) (TmVarS t) (TmAppl (TmVarS x) (TmVarS x))) =
-  TmForA (Some x) (TmVarS t) (TmAppl (TmVarS x) TmVoid). (* Note that we ignore the first `x`! *)
-Proof. intros. simpl. rewrite eqb_refl. apply eqb_neq in H. rewrite H. reflexivity. Qed.
+Example subst_lambda_x : forall t x y, t <> x ->
+  (* subst x y (\x:t. x x) = \x:t. x y *)
+  subst x y (TmForA (Some x) (TmVarS t) (TmAppl (TmVarS x) (TmVarS x))) =
+  TmForA (Some x) (TmVarS t) (TmAppl (TmVarS x) y). (* Note that we ignore the first `x`! *)
+Proof. intros. simpl. rewrite eqb_refl. apply eqb_neq in H. rewrite H. simpl. reflexivity. Qed.
 
-Example subst_lambda_x_l : forall t x, t <> x ->
-  subst x TmVoid (TmForA (Some x) (TmVarS t) (TmAppl (TmAppl (TmVarS x) (TmVarS x)) (TmVarS x))) =
-  TmForA (Some x) (TmVarS t) (TmAppl (TmAppl (TmVarS x) TmVoid) (TmVarS x)).
-Proof. intros. simpl. rewrite eqb_refl. apply eqb_neq in H. rewrite H. reflexivity. Qed.
+Example subst_lambda_x_l : forall t x y, t <> x ->
+  subst x y (TmForA (Some x) (TmVarS t) (TmAppl (TmAppl (TmVarS x) (TmVarS x)) (TmVarS x))) =
+  TmForA (Some x) (TmVarS t) (TmAppl (TmAppl (TmVarS x) y) (TmVarS x)).
+Proof. intros. simpl. rewrite eqb_refl. apply eqb_neq in H. rewrite H. simpl. reflexivity. Qed.
 
-Example subst_lambda_x_r : forall t x, t <> x ->
-  subst x TmVoid (TmForA (Some x) (TmVarS t) (TmAppl (TmVarS x) (TmAppl (TmVarS x) (TmVarS x)))) =
-  TmForA (Some x) (TmVarS t) (TmAppl (TmVarS x) (TmAppl TmVoid (TmVarS x))).
-Proof. intros. simpl. rewrite eqb_refl. apply eqb_neq in H. rewrite H. reflexivity. Qed.
+Example subst_lambda_x_r : forall t x y, t <> x ->
+  subst x y (TmForA (Some x) (TmVarS t) (TmAppl (TmVarS x) (TmAppl (TmVarS x) (TmVarS x)))) =
+  TmForA (Some x) (TmVarS t) (TmAppl (TmVarS x) (TmAppl y (TmVarS x))).
+Proof. intros. simpl. rewrite eqb_refl. apply eqb_neq in H. rewrite H. simpl. reflexivity. Qed.
 
-Theorem subst_fv : forall x y t,
-  fv (subst x y t) =
-  match splitrm (eqb x) (fv t) with
-  | None => fv t
-  | Some (pre, post) => pre ++ fv y ++ post
-  end.
+Example subst_scope : forall x y,
+  (* In which `(\x. 0) x` should not let the bound `x` escape its scope and capture the second (free) `x`. *)
+  subst x y (TmAppl (TmForA (Some x) TmVoid TmVoid) (TmVarS x)) = (TmAppl (TmForA (Some x) TmVoid TmVoid) y).
+Proof. intros. simpl. rewrite eqb_refl. simpl. reflexivity. Qed.
+
+Example subst_arg_cant_be_its_own_type : forall x y,
+  subst x y (TmForA (Some x) (TmVarS x) TmVoid) = (TmForA (Some x) y TmVoid).
+Proof. intros. simpl. rewrite eqb_refl. simpl. reflexivity. Qed.
+
+Example subst_many_times_in_types : forall x y,
+  subst x y (TmForA None (TmVarS x) (TmForA None (TmVarS x) TmVoid)) = (TmForA None y (TmForA None y TmVoid)).
+Proof. intros. simpl. rewrite eqb_refl. simpl. reflexivity. Qed.
+
+Example subst_type_shadowing : forall x y,
+  subst x y (TmForA (Some x) (TmVarS x) (TmForA None (TmVarS x) TmVoid)) = (TmForA (Some x) y (TmForA None (TmVarS x) TmVoid)).
+Proof. intros. simpl. rewrite eqb_refl. simpl. reflexivity. Qed.
+
+Theorem remove_all_partition_pf : forall x hi lo,
+  remove_all x (partition_pf eqb hi lo) = partition_pf eqb (remove_all x hi) (remove_all x lo).
 Proof.
-  intros. rewrite splitrm_fast_slow. simpl in *. generalize dependent x. generalize dependent y.
-  induction t; intros; simpl in *; try reflexivity; repeat rewrite slow_down in *.
-  - destruct (eqb_spec x id). { subst. rewrite eqb_refl. rewrite app_nil_r. reflexivity. }
-    apply eqb_neq in n. rewrite eqb_sym in n. rewrite n. reflexivity.
-  - destruct arg as [arg |]; simpl in *.
+  intros. repeat rewrite partition_pf_fast_slow. generalize dependent x. generalize dependent lo.
+  induction hi; intros; simpl in *. { reflexivity. }
+  destruct (existsb (eqb a) lo) eqn:El; simpl. {
+    rewrite IHhi. destruct (eqb_spec x a). { reflexivity. } simpl.
+    rewrite existsb_remove_all_neq; [| intro C; subst; apply n; reflexivity]. rewrite El. reflexivity. }
+  destruct (existsb (eqb a) hi) eqn:Eh; simpl. {
+    rewrite IHhi. destruct (eqb_spec x a). { reflexivity. } simpl.
+    repeat (rewrite existsb_remove_all_neq; [| intro C; subst; apply n; reflexivity]). rewrite El. rewrite Eh. reflexivity. }
+  destruct (eqb_spec x a). { apply IHhi. } simpl.
+  repeat (rewrite existsb_remove_all_neq; [| intro C; subst; apply n; reflexivity]).
+  rewrite El. rewrite Eh. simpl. f_equal. apply IHhi.
+Qed.
+
+Inductive TryRemove {T} (x : T) : list T -> list T -> Prop :=
+  | TryRemoveNil :
+      TryRemove x [] []
+  | TryRemoveEq : forall tl,
+      TryRemove x (x :: tl) tl
+  | TryRemoveNeq : forall hd tl tl',
+      x <> hd ->
+      TryRemove x tl tl' ->
+      TryRemove x (hd :: tl) (hd :: tl')
+  .
+
+Lemma try_remove_xor : forall {T} x pre post,
+  @TryRemove T x pre post ->
+  ((In x pre /\ pre <> post) \/ (~In x pre /\ pre = post)).
+Proof.
+  intros. induction H; simpl in *.
+  - right. split. { intros []. } reflexivity.
+  - left. split. { left. reflexivity. } intro C. induction tl. { discriminate C. } invert C. apply IHtl in H1 as [].
+  - destruct IHTryRemove as [[IH1 IH2] | [IH1 IH2]].
+    + left. split. { right. assumption. } intro C. invert C. apply IH2. reflexivity.
+    + right. split. { intros [C | C]. { subst. apply H. reflexivity. } apply IH1 in C as []. } f_equal. assumption.
+Qed.
+
+(*
+Theorem subst_fv : forall x y t,
+  Closed y ->
+  StructurallyClosed y -> (* this is clunky but `Closed y -> StructurallyClosed y` is either insanely difficult or false *)
+  TryRemove x (fv t) (fv (subst x y t)).
+Proof.
+  intros x y t Hf Hs. simpl in *. generalize dependent x. generalize dependent y.
+  induction t; intros; simpl in *; try solve [repeat constructor]; repeat rewrite slow_down in *.
+  - destruct (eqb_spec id x); [subst; apply reflect_fv in Hf; simpl; rewrite Hf |]; repeat constructor.
+    intro C. subst. apply n. reflexivity.
+  - specialize (IHt1 _ Hf Hs). specialize (IHt2 _ Hf Hs).
+    destruct (subst_hole_acc (if eq_opt arg (Some x) then Some 1 else Some 0) x t2) as [scurry ac1] eqn:Es.
+    simpl in *. rewrite slow_down. destruct arg as [arg |]; simpl in *.
     + admit.
-    + destruct (subst_hole_acc (Some 0) x t2) as [scurry ac1] eqn:E. simpl in *. rewrite slow_down.
-      rewrite <- splitrm_fast_slow. rewrite splitrm_app. repeat rewrite splitrm_fast_slow.
-      clear IHt1 IHt2.
+    + assert (A := IHt2 x). rewrite Es in A. simpl in A. induction A.
+
+      assert (X := A). apply try_remove_xor in X as [[X1 X2] | [X1 X2]].
+      * admit.
+      * rewrite <- X2. 
+
+  - specialize (IHt1 _ Hf Hs). specialize (IHt2 _ Hf Hs).
+    destruct (subst_hole_acc (if eq_opt arg (Some x) then Some 1 else Some 0) x t2) as [scurry ac1] eqn:E.
+    simpl. rewrite slow_down. destruct arg as [arg |]; simpl in *; rewrite remove_all_app;
+    repeat rewrite <- partition_pf_fast_slow; rewrite remove_all_partition_pf; repeat rewrite partition_pf_fast_slow. 2: {
+      assert (A := IHt2 x). rewrite E in A. simpl in A. rewrite A. f_equal. f_equal. apply structural_subst_fv. assumption. }
+    destruct (eqb_spec arg x). 2: { assert (A := IHt2 x). rewrite E in A. simpl in A. rewrite A.
+      destruct (fv t2) eqn:Ef2; simpl. { f_equal. f_equal. apply structural_subst_fv. assumption. }
+      destruct (eqb_spec x s); subst; simpl in *. {
+        rewrite eqb_refl in A. apply eqb_neq in n. rewrite n. simpl. rewrite eqb_refl.
+        destruct (remove_all s l); simpl. { f_equal. f_equal. apply structural_subst_fv. assumption. }
+        destruct (eqb_spec arg s0).
 Qed.
 
 Fixpoint count_slow {T} (f : T -> bool) li :=
@@ -132,31 +223,6 @@ Proof.
     + Print partition_pf_slow. 
 Qed.
 
-Theorem grand_unified_subst_fv : forall t s,
-  grand_unified_subst t = Some s ->
-  fv t = map fst s.
-Proof.
-  induction t; intros; simpl in *; try solve [invert H; reflexivity]; repeat rewrite slow_down in *;
-  repeat rewrite structural_grand_unified_subst_fv in *.
-  - destruct (grand_unified_subst t2) as [s2 |] eqn:Es2; [| discriminate H].
-    specialize (IHt2 _ eq_refl). repeat rewrite IHt2 in *. rewrite slow_down_kv in H.
-    destruct (partition_kv_pf_slow eqb eq_hole
-      (smap (fun h : hole => HolePackTy id arg h t2) (structural_grand_unified_subst t1))
-      (smap (HolePackCurry id arg t1) match arg with Some a => remove_key_if_head a s2 | None => s2 end)
-    ) eqn:Ep; invert H; simpl in *. rewrite <- partition_kv_pf_fast_slow in Ep. eapply partition_kv_pf_works in Ep.
-    Search (PartitionKV _ _ _ -> _).
-    destruct arg. 2: {
-      rewrite <- partition_pf_fast_slow. rewrite <- (map_fst_partition_pf _ _ _ _ fst_cmp_eqb).
-      rewrite map_distr. rewrite map_fst_smap. f_equal. Search fst_cmp.
-    Search partition_pf.
-    clear H.
-  rewrite map_distr; try rewrite (map_fst_partition_pf _ _ _ _ fst_cmp_eqb); repeat rewrite map_fst_smap;
-  repeat rewrite IHt1; repeat rewrite IHt2; [| | reflexivity]; rewrite structural_grand_unified_subst_fv;
-  (destruct arg; [| reflexivity]); repeat rewrite partition_pf_fast_slow; (destruct (grand_unified_subst t2); [reflexivity |]);
-  destruct p as [v f]; simpl; destruct (eqb s v); reflexivity.
-Qed.
-(* WOOHOOOOOOOOOOOOOOO *)
-
 Lemma remove_key_if_head_incl : forall {T} x (li : list (string * T)),
   incl (remove_key_if_head x li) li.
 Proof.
@@ -172,96 +238,31 @@ Proof.
   destruct a as [k1 v1]. destruct a0 as [k2 v2]. destruct H; [| right; apply (IHhi _ _ H)].
   left. assumption.
 Qed.
+*)
 
-Theorem grand_unified_subst_id : forall t,
-  let P := fun p : _ * _ => let (x, f) := p in fill f (TmVarS x) = t in
-  Forall P (grand_unified_subst t).
+Lemma subst_id_deconstructed : forall acc x t,
+  sfill (fst (subst_hole_acc acc x t)) (TmVarS x) = t.
 Proof.
-  induction t as [| | | | id arg a IHa b IHb | arg a IHa b IHb | a IHa b IHb]; simpl in *; repeat constructor; [| |
-    apply Forall_app; split; apply Forall_smap; (eapply Forall_impl; [| try apply IHa; apply IHb]);
-    intros; destruct a0; simpl; rewrite H; reflexivity]; repeat rewrite slow_down; destruct arg;
-  apply Forall_app; (split; [eapply incl_Forall; [apply incl_partition_pf_fst |] |]);
-  apply Forall_smap; try (eapply incl_Forall; [apply remove_key_if_head_incl |]);
-  (eapply Forall_impl; [| try apply structural_grand_unified_subst_id; apply IHb]);
-  intros; destruct a0; simpl; rewrite H; reflexivity.
+  intros. generalize dependent acc. generalize dependent x. induction t; intros; simpl in *; try reflexivity.
+  - destruct (eqb_spec id x); [subst |]; destruct acc; [destruct n | | |]; reflexivity.
+  - destruct (subst_hole_acc (if eq_opt arg (Some x) then option_map S acc else acc) x t2) as [scurry ac1] eqn:E.
+    simpl in *. f_equal. { destruct acc; [destruct n |]; try reflexivity. apply structural_subst_id. }
+    assert (A := IHt2 x (if eq_opt arg (Some x) then option_map S acc else acc)). rewrite E in A. simpl in A. assumption.
+  - destruct (subst_hole_acc (if eq_opt arg (Some x) then option_map S acc else acc) x t2) as [scurry ac1] eqn:E.
+    simpl in *. f_equal. { destruct acc; [destruct n |]; try reflexivity. apply structural_subst_id. }
+    assert (A := IHt2 x (if eq_opt arg (Some x) then option_map S acc else acc)). rewrite E in A. simpl in A. assumption.
+  - destruct (subst_hole_acc acc x t1) as [sf tmp] eqn:E1. destruct tmp; [destruct acc |];
+    [destruct (subst_hole_acc (checked_sub n n0) x t2) as [sz out] eqn:E2 | |];
+    try destruct (subst_hole_acc None x t2) as [sz out] eqn:E2; simpl in *;
+    eassert (A1 := IHt1 _ _); eassert (A2 := IHt2 _ _); rewrite E1 in A1; rewrite E2 in A2;
+    simpl in *; rewrite A1; rewrite A2; reflexivity.
 Qed.
 
-Theorem subst_id : forall x t s,
-  subst x (TmVarS x) t = Some s ->
-  s = t.
-Proof.
-  intros. unfold subst in *. destruct (pair_lookup x (grand_unified_subst t)) eqn:Ep; invert H.
-  eapply pair_lookup_Forall in Ep; [| apply grand_unified_subst_id]. assumption.
-Qed.
+Theorem subst_id : forall x t,
+  subst x (TmVarS x) t = t.
+Proof. apply subst_id_deconstructed. Qed.
 
-Variant DecapitateK {K V} (k : K) : list (K * V) -> list (K * V) -> Prop :=
-  | DecapitateKNil :
-      DecapitateK k [] []
-  | DecapitateKConsEq : forall hv tl,
-      DecapitateK k ((k, hv) :: tl) tl
-  | DecapitateKConsNEq : forall hk hv tl,
-      k <> hk ->
-      DecapitateK k ((hk, hv) :: tl) ((hk, hv) :: tl)
-  .
-
-Theorem reflect_decapitate_k : forall {V} k li post,
-  remove_key_if_head k li = post <-> @DecapitateK _ V k li post.
-Proof.
-  split; intros.
-  - subst. destruct li; simpl in *. { constructor. }
-    destruct p. destruct (eqb_spec k s). { subst. constructor. } constructor. assumption.
-  - destruct H; simpl in *; [| rewrite eqb_refl | apply eqb_neq in H; rewrite H]; reflexivity.
-Qed.
-
-Inductive GrandUnifiedSubst : term -> list (string * hole) -> Prop :=
-  | GUSVoid :
-      GrandUnifiedSubst TmVoid []
-  | GUSStar : forall univ,
-      GrandUnifiedSubst (TmStar univ) []
-  | GUSVarS : forall s,
-      GrandUnifiedSubst (TmVarS s) [(s, HoleHere)]
-  | GUSAtom : forall id,
-      GrandUnifiedSubst (TmAtom id) []
-  | GUSPack : forall id arg ty curry sty scurry scurry_orig pf s,
-      GrandUnifiedSubst ty sty ->
-      GrandUnifiedSubst curry scurry_orig ->
-      match arg with
-      | None => eq
-      | Some a => DecapitateK a
-      end scurry_orig scurry ->
-      PartitionKV pf sty scurry ->
-      s = smap (fun h => HolePackTy id arg h curry) pf ++ smap (HolePackCurry id arg ty) scurry ->
-      GrandUnifiedSubst (TmPack id arg ty curry) s
-  | GUSForA : forall arg ty body sty sbody sbody_orig pf s,
-      GrandUnifiedSubst ty sty ->
-      GrandUnifiedSubst body sbody_orig ->
-      match arg with
-      | None => eq
-      | Some a => DecapitateK a
-      end sbody_orig sbody ->
-      PartitionKV pf sty sbody ->
-      s = smap (fun h => HoleForATy arg h body) pf ++ smap (HoleForABody arg ty) sbody ->
-      GrandUnifiedSubst (TmForA arg ty body) s
-  | GUSAppl : forall f x sf sx s,
-      GrandUnifiedSubst f sf ->
-      GrandUnifiedSubst x sx ->
-      s = smap (fun h => HoleApplF h x) sf ++ smap (HoleApplX f) sx ->
-      GrandUnifiedSubst (TmAppl f x) s
-  .
-
-Theorem reflect_structural_grand_unified_subst : forall t s,
-  grand_unified_subst t = s <-> GrandUnifiedSubst t s.
-Proof.
-  split; intros.
-  - generalize dependent s. induction t; intros; subst; simpl in *; try solve [constructor]; try rewrite slow_down.
-    + econstructor.
-      * apply IHt1. reflexivity.
-      * apply IHt2. reflexivity.
-      * shelve.
-      * apply (partition_pf_works). Search (partition_pf).
-      * f_equal.
-
-    econstructor. ; try apply IHt1; try apply IHt2; try reflexivity; (destruct arg; [apply reflect_purge_k |]); reflexivity.
-  - induction H; subst; simpl in *; f_equal; (destruct arg; [| subst; reflexivity]);
-    apply reflect_purge_k in H1; subst; reflexivity.
-Qed.
+(* TODO: `Prop` versions
+Definition Subst (x : string) (y t t' : term) := exists h, SubstHole x t h /\ Fill h y t'.
+Arguments Subst/ x y t t'.
+*)
