theories/Static.v
@@ -1,0 +1,58 @@
+From Lang Require Import
+  FreeVariables
+  Invert
+  StructuralFreeVariables
+  Terms.
+
+(* Static, i.e. not (anywhere) dependently typed.
+ * Note that this is exactly the same under structural and non-structural interpretation!
+ * In either case, we'd use `StructurallyClosed` and `StructurallyStatic` at the type level,
+ * and all else is identical boilerplate. *)
+Inductive Static : term -> Prop :=
+  | StaticVoid :
+      Static TmVoid
+  | StaticStar : forall univ,
+      Static (TmStar univ)
+  | StaticVarS : forall x,
+      Static (TmVarS x)
+  | StaticAtom : forall id,
+      Static (TmAtom id)
+  | StaticPack : forall id arg ty curry,
+      Static (TmForA arg ty curry) ->
+      Static (TmPack id arg ty curry)
+  | StaticForA : forall arg ty body,
+      (* TODO: change this to accept ONLY `TmForA None ...` (note the `None`), then update typing rules s.t. types have `None` iff `curry`/`body` doesn't have `arg` free *)
+      StructurallyClosed ty -> (* this is the only line that really matters. NOTE: no matter the context. *)
+      Static ty -> (* TODO: Is this necessary? *)
+      Static body ->
+      Static (TmForA arg ty body)
+  | StaticAppl : forall f x,
+      Static f ->
+      Static x ->
+      Static (TmAppl f x)
+  .
+
+Fixpoint static t :=
+  match t with
+  | TmVoid
+  | TmStar _
+  | TmVarS _
+  | TmAtom _ =>
+      true
+  | TmPack _ _ ty curry
+  | TmForA _ ty curry =>
+      andb (andb (structurally_closed ty) (static ty)) (static curry)
+  | TmAppl f x =>
+      andb (static f) (static x)
+  end.
+
+Theorem reflect_static : forall t,
+  Bool.reflect (Static t) (static t).
+Proof.
+  induction t; repeat constructor; simpl in *; invert IHt1; invert IHt2;
+  repeat rewrite Bool.andb_true_r; repeat rewrite Bool.andb_false_r;
+  try (constructor; intro C; invert C; try contradiction; invert H4; contradiction); [| | repeat constructor; assumption];
+  destruct (structural_fv t1) eqn:E; assert (A := E); simpl in E; rewrite E; repeat constructor;
+  try apply reflect_structural_fv; try assumption; intro C; invert C; [invert H4; rename H7 into H6 |];
+  apply reflect_structural_fv in H6; rewrite A in H6; discriminate H6.
+Qed.
